push

tests/lean/run/cbv1.lean
@@ -1,5 +1,4 @@
-import Std.Data.TreeMap
-import Std.Data.DTreeMap
+import Std
 
 def function (n : Nat) : Nat := match n with
   | 0 => 0 + 1
@@ -87,6 +86,70 @@ def testFun (l : List Nat) : Nat := Id.run do
 
 -- Would be nice if we perfomed zeta reduction
 example : testFun [1,2,3,4,5] = 5 := by
+  conv =>
+    lhs
+    cbv
+
+set_option trace.Meta.Tactic.cbv true
+
+example : "a" ++ "a" = "aa" := by
+  conv =>
+    lhs
+    cbv
+
+#check String.utf8EncodeChar.eq_1
+
+theorem concat_test : "ab".length + "ab".length = ("ab" ++ "ab").length := by
+  conv =>
+    lhs
+    cbv
+  conv =>
+    rhs
+    cbv
+
+
+
+structure myStruct where
+  a : HDiv Nat Nat Nat
+
+example : ({a := instHDiv} : myStruct) = sorry := by
+  conv =>
+    lhs
+    cbv
+
+example :  instHDiv.1 119 262144  = sorry := by
+  conv =>
+    lhs
+    cbv
+
+theorem std_test2 : (((Std.TreeMap.empty : Std.TreeMap Nat Nat).insert 2 4).toList ++ [(5, 6)]).reverse = [(5,6), (2,4)] := by
+  conv =>
+    lhs
+    cbv
+
+#print std_test2
+
+example : "wojtek".1 = sorry := by
+  conv =>
+    lhs
+    cbv
+
+def h := ()
+
+example : h = () := by
+  conv =>
+    lhs
+    -- Does not unfold the constant, we need to figure out what is a good way of dealing with it
+    cbv
+
+
+example : ((Std.HashMap.emptyWithCapacity : Std.HashMap Nat Nat).insert 4 3).contains 4 = sorry := by
+  conv =>
+    lhs
+    cbv
+
+set_option trace.Meta.Tactic.cbv true
+example : 2 + 2 = 4 := by
   conv =>
     lhs
     cbv
